Printing.thy
@@ -80,9 +80,6 @@ lemma print_ce [simp]: "hcontains h x \<Longrightarrow>
     print_ceclosure (hlookup h x) = print_hclosure (hlookup (unchain_heap h env) x)"
   by (cases "hlookup h x") simp_all
 
-lemma [simp]: "print_ceclosure (flatten_closure' c) = print_ceclosure c"
-  by (induction c) simp_all
-
 lemma print_a [simp]: "3 dvd x \<Longrightarrow> Suc x < hp \<Longrightarrow> 
   print_uval (pseudoreg_map \<circ> assm_hp cd h hp) x = print_uval h x"
 proof (induction "h x")
@@ -92,6 +89,22 @@ proof (induction "h x")
   moreover from Suc have "Suc x mod 3 = 1" by presburger
   ultimately show ?case by (simp add: assm_hp_lemma1 assm_hp_lemma2 split: nat.splits)
 qed (simp_all add: assemble_heap_def)
+
+fun get_closure :: "nat heap \<Rightarrow> ptr \<Rightarrow> closure\<^sub>v" where
+  "get_closure h p = (case hlookup h p of
+      0 \<Rightarrow> Lam\<^sub>v (hlookup h (Suc p)) (hlookup h (Suc (Suc p)))
+    | Suc _ \<Rightarrow> Const\<^sub>v (hlookup h (Suc p)))"
+
+primrec flatten_closure' :: "closure\<^sub>v \<Rightarrow> closure\<^sub>v" where
+  "flatten_closure' (Const\<^sub>v k) = Const\<^sub>v k"
+| "flatten_closure' (Lam\<^sub>v p pc) = Lam\<^sub>v (2 * p) pc"
+
+lemma [simp]: "print_ceclosure (flatten_closure' c) = print_ceclosure c"
+  by (induction c) simp_all
+
+lemma [simp]: "hcontains h v \<Longrightarrow> 
+    get_closure (flatten_values h) (3 * v) = flatten_closure' (hlookup h v)"
+  by (simp split: closure\<^sub>v.splits)
 
 lemma print_u [simp]: "print_uval h p = print_ceclosure (get_closure (H h hp) p)"
   by (cases "h p") simp_all
